theories/Blacks_Rule_Ref.thy
@@ -2,15 +2,31 @@ section \<open>Black's Rule\<close>
 
 theory Blacks_Rule_Ref
   imports"Verified_Voting_Rule_Construction.Blacks_Rule"
-          Pairwise_Majority_Rule_Ref
-          Borda_Rule_Ref
+          "Compositional_Structures/Basic_Modules/Condorcet_Module_Ref"  
+          "Compositional_Structures/Basic_Modules/Borda_Module_Ref"  
+          "Compositional_Structures/Sequential_Composition_Ref"
 begin
 
 
 subsection \<open>Definition\<close>
 
-definition blacks_rule_sep where
-  "blacks_rule_sep \<equiv> (pairwise_majority_rule_sep) \<triangleright>sep borda_rule_sep"
+sepref_definition blacks_rule_direct is "uncurry (seq_opt condorcet borda)"
+  :: "elec_mod_sep_rel nat_assn"
+  unfolding seq_opt_def
+  apply sepref_dbg_keep
+  done
+
+lemmas opt_seq_blacks = seq_opt_correct[OF condorcet_sound borda_sound]
+lemmas opt_blacks_correct_aux = blacks_rule_direct.refine[FCOMP opt_seq_blacks]
+
+lemma blacks_direct_correct:
+  shows "(uncurry blacks_rule_direct, uncurry (RETURN oo (blacks_rule:: (nat Electoral_Module))))
+  \<in> elec_mod_sep_rel nat_assn"
+  unfolding blacks_rule.simps
+  using  opt_blacks_correct_aux  prod_rel_id_simp set_rel_id hr_comp_Id2
+  by metis
+
+declare opt_pmc_correct [sepref_fr_rules]
 
 
 end
