theories/Pairwise_Majority_Rule_Ref.thy
@@ -26,7 +26,24 @@ lemma  pairwise_majority_rule_correct [sepref_fr_rules]:
   unfolding pairwise_majority_rule_sep_def pairwise_majority_rule.simps 
     using pairwise_majority_rule_impl.elector_sep_correct .
 
+sepref_definition pairwise_majority_rule_direct is "uncurry (seq_opt condorcet elect_module
+  )"
+  :: "elec_mod_sep_rel nat_assn"
+  unfolding seq_opt_def
+  apply sepref_dbg_keep
+  done
 
-export_code clist pairwise_majority_rule_sep in Scala_imp
+lemmas opt_seq_pmc = seq_opt_correct[OF condorcet_sound elect_mod_sound]
+lemmas opt_seq_pmct_aux = pairwise_majority_rule_direct.refine[FCOMP opt_seq_pmc]
+
+lemma opt_pmc_correct:
+  shows "(uncurry pairwise_majority_rule_direct, uncurry (RETURN oo (pairwise_majority_rule:: (nat Electoral_Module))))
+  \<in> elec_mod_sep_rel nat_assn"
+  unfolding pairwise_majority_rule.simps elector.simps 
+  using  opt_seq_pmct_aux  prod_rel_id_simp set_rel_id hr_comp_Id2
+  by metis
+
+
+export_code clist convert_list_to_hash_set pairwise_majority_rule_direct in Scala_imp
 
 end
